tests/ll/call-cast.ll
@@ -1,0 +1,11 @@
+define i64 @g0(i64 %arg) {
+    %res = add i64 %arg, 3
+    ret i64 %res
+}
+
+define  i64 @main() {
+    %fint = ptrtoint i64 (i64)* @g0 to i64
+    %fptr = inttoptr i64 %fint to i64 (i64)*
+    %res = call i64 (i64) %fptr(i64 0)
+    ret i64 %res
+}
