src/coq/Semantics/Denotation.v
@@ -28,6 +28,7 @@ From Vellvm Require Import
      Numeric.Integers
      Numeric.Floats
      Utilities
+     Utils.IntMaps
      Syntax
      Semantics.VellvmIntegers
      Semantics.LLVMEvents
@@ -617,10 +618,15 @@ Module Denotation (LP : LLVMParams) (MP : MemoryParams LP) (Byte : ByteModule LP
          that life in the "right" injection of the [_CFG_INTERNAL] effect
    *)
 
-  Definition lookup_defn {B} := @assoc dvalue B _.
+  Definition lookup_defn (dv : dvalue) (m : IntMap function_denotation) : option function_denotation
+    := match dv with
+       | DVALUE_Addr addr =>
+           lookup (PTOI.ptr_to_int addr) m
+       | _ => None
+       end.
 
   Definition denote_mcfg
-             (fundefs:list (dvalue * function_denotation)) (dt : dtyp)
+             (fundefs:IntMap function_denotation) (dt : dtyp)
              (f_value : uvalue) (args : list uvalue) : itree L0 uvalue :=
     @mrec CallE (ExternalCallE +' _)
           (fun T call =>
